Iris/Iris/BI/WeakestPre.lean
@@ -1,0 +1,146 @@
+module
+
+public import Iris.Std.CoPset
+public import Iris.BI
+public meta import Iris.BI
+public import Iris.BI.BIBase
+public meta import Iris.Std.Rewrite
+public import Std
+meta import Lean
+public import Lean
+
+public import Iris.BI.BI
+public import Iris.BI.Classes
+public import Iris.BI.DerivedLaws
+public import Iris.BI.DerivedLawsLater
+public import Iris.BI.Extensions
+public import Iris.BI.SIProp
+public meta import Iris.Std.RocqPorting
+
+public section
+
+namespace Iris
+
+open Lean
+
+inductive Stuckness where
+| NotStuck
+| MaybeStuck
+
+namespace Stuckness
+
+@[simp]
+instance instLE: LE Stuckness where
+  le x y := ¬ (x = .MaybeStuck ∧ y = .NotStuck)
+
+instance : Std.IsPreorder Stuckness where
+  le_refl  := by grind only [Stuckness, LE.le, instLE]
+  le_trans := by grind only [Stuckness, LE.le, instLE]
+
+@[simp] theorem le_MaybeStuck {s : Stuckness} : s ≤ MaybeStuck := by
+  cases s <;> grind only [Stuckness, LE.le, instLE]
+
+@[simp] theorem NotSuck_le {s : Stuckness} : NotStuck ≤ s := by
+  cases s <;> grind only [Stuckness, LE.le, instLE]
+
+end Stuckness
+
+class Wp (PROP Expr : Type _) (Val : outParam (Type _)) (A : Type _) where
+  wp : A → CoPset → Expr → (Val → PROP) → PROP
+
+class TotalWP (PROP Expr) (Val : outParam (Type _)) (A : Type _) where
+  totalWp : A → CoPset → Expr → (Val → PROP) → PROP
+
+syntax wpExpr :=
+  term:max (" @ " term:max (" ; " term:max) <|> ((" ? ")? )) <|> (" ? ")?
+
+declare_syntax_cat wpPostcondInner
+syntax ident ", " term : wpPostcondInner
+syntax term : wpPostcondInner
+
+declare_syntax_cat wpPostcond
+-- Avoids conflicts with
+-- example {a : PUnit.{i}} : PUnit.{i} := a
+--                      ^^
+-- see: https://github.com/leanprover-community/iris-lean/pull/393
+syntax " {" "{ " wpPostcondInner " }" "} " : wpPostcond
+syntax " [" "{ " wpPostcondInner " }" "] " : wpPostcond
+syntax " ⦃ " wpPostcondInner " ⦄ " : wpPostcond
+syntax " 〖 " wpPostcondInner " 〗 "  : wpPostcond
+
+syntax (name := wp) "WP " wpExpr wpPostcond : term
+
+open Lean in
+meta def parseWpExpr : Lean.TSyntax ``wpExpr → Lean.MacroM (TSyntax `term × TSyntax `term × TSyntax `term) := fun
+  | `(wpExpr| $e @ $s ; $E) =>
+    return (e, s, E)
+  | `(wpExpr| $e @ $E) =>
+    return (e, ←`(Stuckness.NotStuck), E)
+  | `(wpExpr| $e @ $E ?) =>
+    return (e, ←`(Stuckness.MaybeStuck), E)
+  | `(wpExpr| $e:term) =>
+    return (e, ←`(Stuckness.NotStuck), ←`(⊤))
+  | `(wpExpr| $e:term ?) =>
+    return (e, ←`(Stuckness.MaybeStuck), ←`(⊤))
+  | _ => Lean.Macro.throwUnsupported
+
+open Lean in
+meta def parseWpPostcondInner (stx : TSyntax `wpPostcondInner) : MacroM (TSyntax `term) := do
+  match stx with
+  | `(wpPostcondInner| $v:ident, $Φ:term) => `(fun $v => iprop($Φ))
+  | `(wpPostcondInner| $Φ:term) => return iprop(Φ)
+  | _ => Macro.throwUnsupported
+
+open Lean in
+meta def parseWpPostcond (stx : TSyntax `wpPostcond) : MacroM (TSyntax `term × Bool) := do
+  match stx with
+  | `(wpPostcond| {{ $inner:wpPostcondInner }})
+  | `(wpPostcond| ⦃ $inner:wpPostcondInner ⦄) =>
+    return (←parseWpPostcondInner inner, false)
+  | `(wpPostcond| [{ $inner:wpPostcondInner }])
+  | `(wpPostcond| 〖 $inner:wpPostcondInner 〗) =>
+    return (←parseWpPostcondInner inner, true)
+  | _ => Macro.throwUnsupported (α := TSyntax `term × Bool)
+
+@[macro wp]
+meta def wpMacro : Lean.Macro := fun stx => do
+  match stx with
+  | `(WP $expr $postcond) =>
+    let (e, s, E) ← parseWpExpr expr
+    let (Φ, useTotal?) ← parseWpPostcond postcond
+    if useTotal? then
+      `(TotalWP.totalWp $s $E $e $Φ)
+    else
+      `(Wp.wp $s $E $e $Φ)
+  | _ => Lean.Macro.throwUnsupported
+
+meta def unexpandWpPostcondInner : TSyntax `term → PrettyPrinter.UnexpandM (TSyntax `wpPostcondInner)
+  | `(fun $v:ident => iprop($Φ:term)) => `(wpPostcondInner|$v:ident, $Φ:term)
+  | `(iprop($Φ:term)) => `(wpPostcondInner| $Φ:term)
+  | `(fun $v:ident => $Φ:term) => `(wpPostcondInner|$v:ident, $Φ:term)
+  | `($Φ:term) => `(wpPostcondInner| $Φ:term)
+
+open Lean in
+meta def makeWpExpr (s E e : TSyntax `term) : PrettyPrinter.UnexpandM (TSyntax ``wpExpr) := do
+  match s, E with
+  | `(Stuckness.NotStuck), `(⊤) => `(wpExpr| $e:term)
+  | `(Stuckness.NotStuck), E => `(wpExpr| $e:term @ $E:term)
+  | `(Stuckness.MaybeStuck), `(⊤) => `(wpExpr| $e:term ?)
+  | `(Stuckness.MaybeStuck), E => `(wpExpr| $e:term @ $E:term ?)
+  | s, E => `(wpExpr| $e:term @ $s:term ; $E:term)
+
+@[app_unexpander Wp.wp]
+meta def unexpanderWp : PrettyPrinter.Unexpander
+  | `($_wp $s $E $e $Φ) => do
+    let wpExpr ← makeWpExpr s E e
+    let wpPostcondInner ← unexpandWpPostcondInner Φ
+    `(WP $wpExpr {{ $wpPostcondInner }})
+  | _ => throw ()
+
+@[app_unexpander TotalWP.totalWp]
+meta def unexpanderTotalWp : PrettyPrinter.Unexpander
+  | `($_wp $s $E $e $Φ) => do
+    let wpExpr ← makeWpExpr s E e
+    let wpPostcondInner ← unexpandWpPostcondInner Φ
+    `(WP $wpExpr [{ $wpPostcondInner }])
+  | _ => throw ()
