Iris/Iris/Instances/IProp/Instance.lean
@@ -16,6 +16,9 @@ namespace Iris
 
 open COFE
 
+@[ext]
+theorem IProp.ext {P Q : IProp GF} : P ⊣⊢ Q → P = Q := OFE.Leibniz.eq_of_eqv ∘ BI.equiv_iff.mpr
+
 /-- Apply an OFunctor at a fixed type -/
 abbrev COFE.OFunctorPre.ap (F : OFunctorPre) (T : Type _) [OFE T] :=
   F T T
